pcuic/theories/PCUICInductiveInversion.v
@@ -1,0 +1,707 @@
+(* Distributed under the terms of the MIT license.   *)
+Set Warnings "-notation-overridden".
+
+Require Import Equations.Prop.DepElim.
+From Coq Require Import Bool String List Lia Arith.
+From MetaCoq.Template Require Import config utils.
+From MetaCoq.PCUIC Require Import PCUICAst PCUICAstUtils
+     PCUICLiftSubst PCUICUnivSubst PCUICTyping PCUICWeakeningEnv PCUICWeakening
+     PCUICSubstitution PCUICClosed PCUICCumulativity PCUICGeneration PCUICReduction
+     PCUICEquality PCUICConfluence PCUICParallelReductionConfluence
+     PCUICContextConversion PCUICUnivSubstitution
+     PCUICConversion PCUICInversion PCUICContexts PCUICArities
+     PCUICParallelReduction PCUICCtxShape PCUICSpine PCUICInductives PCUICValidity.
+     
+Close Scope string_scope.
+
+Require Import ssreflect. 
+
+Set Asymmetric Patterns.
+Set SimplIsCbn.
+
+From Equations Require Import Equations.
+
+Ltac pcuic := intuition eauto 5 with pcuic ||
+  (try solve [repeat red; cbn in *; intuition auto; eauto 5 with pcuic || (try lia || congruence)]).
+
+(** Inversion principles on inductive/coinductives types following from validity. *)
+
+Lemma declared_constructor_valid_ty {cf:checker_flags} Σ Γ mdecl idecl i n cdecl u :
+  wf Σ.1 ->
+  wf_local Σ Γ ->
+  declared_constructor Σ.1 mdecl idecl (i, n) cdecl ->
+  consistent_instance_ext Σ (ind_universes mdecl) u ->
+  isType Σ Γ (type_of_constructor mdecl cdecl (i, n) u).
+Proof.
+  move=> wfΣ wfΓ declc Hu.
+  epose proof (env_prop_typing _ _ validity Σ wfΣ Γ (tConstruct i n u)
+    (type_of_constructor mdecl cdecl (i, n) u)).
+  forward X by eapply type_Construct; eauto.
+  simpl in X.
+  destruct X.
+  2:eauto.
+  destruct i0 as [ctx [s [Hs ?]]].
+  unfold type_of_constructor in Hs.
+  destruct (on_declared_constructor _ declc); eauto.
+  destruct s0 as [cshape [Hsorc Hc]].
+  destruct Hc as [_ chead cstr_eq [cs Hcs] _ _].
+  destruct cshape. rewrite /cdecl_type in cstr_eq.
+  rewrite cstr_eq in Hs. clear -declc Hs.
+  rewrite /subst1 !subst_instance_constr_it_mkProd_or_LetIn
+  !subst_it_mkProd_or_LetIn in Hs.
+  rewrite !subst_instance_constr_mkApps !subst_mkApps in Hs.
+  rewrite !subst_instance_context_length Nat.add_0_r in Hs.
+  rewrite subst_inds_concl_head in Hs.
+  + simpl. destruct declc as [[onm oni] ?].
+    now eapply nth_error_Some_length in oni.
+  + now rewrite !destArity_it_mkProd_or_LetIn destArity_app /= destArity_tInd in Hs.
+Qed.
+
+Lemma type_tFix_inv {cf:checker_flags} (Σ : global_env_ext) Γ mfix idx T : wf Σ ->
+  Σ ;;; Γ |- tFix mfix idx : T ->
+  { T' & { rarg & {f & (unfold_fix mfix idx = Some (rarg, f)) * (Σ ;;; Γ |- f : T') * (Σ ;;; Γ |- T' <= T) }}}%type.
+Proof.
+  intros wfΣ H. depind H.
+  - unfold unfold_fix. rewrite e.
+    specialize (nth_error_all e a0) as [s Hs].
+    specialize (nth_error_all e a1) as [Hty ->].
+    simpl.
+    destruct decl as [name ty body rarg]; simpl in *.
+    clear e.
+    eexists _, _, _. split.
+    + split.
+      * eauto.
+      * eapply (substitution _ _ _ _ [] _ _ wfΣ); simpl; eauto with wf.
+        rename i into hguard. clear -a a0 a1 hguard.
+        pose proof a1 as a1'. apply All_rev in a1'.
+        unfold fix_subst, fix_context. simpl.
+        revert a1'. rewrite <- (@List.rev_length _ mfix).
+        rewrite rev_mapi. unfold mapi.
+        assert (#|mfix| >= #|List.rev mfix|) by (rewrite List.rev_length; lia).
+        assert (He :0 = #|mfix| - #|List.rev mfix|) by (rewrite List.rev_length; auto with arith).
+        rewrite {3}He. clear He. revert H.
+        assert (forall i, i < #|List.rev mfix| -> nth_error (List.rev mfix) i = nth_error mfix (#|List.rev mfix| - S i)).
+        { intros. rewrite nth_error_rev. 1: auto.
+          now rewrite List.rev_length List.rev_involutive. }
+        revert H.
+        generalize (List.rev mfix).
+        intros l Hi Hlen H.
+        induction H.
+        ++ simpl. constructor.
+        ++ simpl. constructor.
+          ** unfold mapi in IHAll.
+              simpl in Hlen. replace (S (#|mfix| - S #|l|)) with (#|mfix| - #|l|) by lia.
+              apply IHAll.
+              --- intros. simpl in Hi. specialize (Hi (S i)). apply Hi. lia.
+              --- lia.
+          ** clear IHAll. destruct p.
+              simpl in Hlen. assert ((Nat.pred #|mfix| - (#|mfix| - S #|l|)) = #|l|) by lia.
+              rewrite H0. rewrite simpl_subst_k.
+              --- clear. induction l; simpl; auto with arith.
+              --- eapply type_Fix; auto.
+                  simpl in Hi. specialize (Hi 0). forward Hi.
+                  +++ lia.
+                  +++ simpl in Hi.
+                      rewrite Hi. f_equal. lia.
+
+    + rewrite simpl_subst_k.
+      * now rewrite fix_context_length fix_subst_length.
+      * reflexivity.
+  - destruct (IHtyping wfΣ) as [T' [rarg [f [[unf fty] Hcumul]]]].
+    exists T', rarg, f. intuition auto.
+    + eapply cumul_trans; eauto.
+    + destruct b. eapply cumul_trans; eauto.
+Qed.
+
+Lemma type_tCoFix_inv {cf:checker_flags} (Σ : global_env_ext) Γ mfix idx T : wf Σ ->
+  Σ ;;; Γ |- tCoFix mfix idx : T ->
+  (allow_cofix = true) * { T' & { rarg & {f & (unfold_cofix mfix idx = Some (rarg, f)) *
+   (Σ ;;; Γ |- f : T') * (Σ ;;; Γ |- T' <= T) }}}%type.
+Proof.
+  intros wfΣ H. depind H.
+  - unfold unfold_cofix. rewrite e. split; auto.
+    specialize (nth_error_all e a1) as Hty.
+    destruct decl as [name ty body rarg]; simpl in *.
+    clear e.
+    eexists _, _, _. split.
+    + split.
+      * eauto.
+      * eapply (substitution _ _ _ _ [] _ _ wfΣ); simpl; eauto with wf.
+        rename i into hguard. clear -a a0 a1 hguard.
+        pose proof a1 as a1'. apply All_rev in a1'.
+        unfold cofix_subst, fix_context. simpl.
+        revert a1'. rewrite <- (@List.rev_length _ mfix).
+        rewrite rev_mapi. unfold mapi.
+        assert (#|mfix| >= #|List.rev mfix|) by (rewrite List.rev_length; lia).
+        assert (He :0 = #|mfix| - #|List.rev mfix|) by (rewrite List.rev_length; auto with arith).
+        rewrite {3}He. clear He. revert H.
+        assert (forall i, i < #|List.rev mfix| -> nth_error (List.rev mfix) i = nth_error mfix (#|List.rev mfix| - S i)).
+        { intros. rewrite nth_error_rev. 1: auto.
+          now rewrite List.rev_length List.rev_involutive. }
+        revert H.
+        generalize (List.rev mfix).
+        intros l Hi Hlen H.
+        induction H.
+        ++ simpl. constructor.
+        ++ simpl. constructor.
+          ** unfold mapi in IHAll.
+              simpl in Hlen. replace (S (#|mfix| - S #|l|)) with (#|mfix| - #|l|) by lia.
+              apply IHAll.
+              --- intros. simpl in Hi. specialize (Hi (S i)). apply Hi. lia.
+              --- lia.
+          ** clear IHAll.
+              simpl in Hlen. assert ((Nat.pred #|mfix| - (#|mfix| - S #|l|)) = #|l|) by lia.
+              rewrite H0. rewrite simpl_subst_k.
+              --- clear. induction l; simpl; auto with arith.
+              --- eapply type_CoFix; auto.
+                  simpl in Hi. specialize (Hi 0). forward Hi.
+                  +++ lia.
+                  +++ simpl in Hi.
+                      rewrite Hi. f_equal. lia.
+    + rewrite simpl_subst_k.
+      * now rewrite fix_context_length cofix_subst_length.
+      * reflexivity.
+  - destruct (IHtyping wfΣ) as [IH [T' [rarg [f [[unf fty] Hcumul]]]]].
+    split; auto.
+    exists T', rarg, f. intuition auto.
+    + eapply cumul_trans; eauto.
+    + destruct b. eapply cumul_trans; eauto.
+Qed.
+
+Lemma on_constructor_subst' {cf:checker_flags} Σ ind mdecl idecl cshape cdecl : 
+  wf Σ -> 
+  declared_inductive Σ mdecl ind idecl ->
+  on_inductive (lift_typing typing) (Σ, ind_universes mdecl) (inductive_mind ind) mdecl ->
+  forall (oib : on_ind_body (lift_typing typing) (Σ, ind_universes mdecl) (inductive_mind ind) mdecl 
+           (inductive_ind ind) idecl)
+        (onc : on_constructor (lift_typing typing) (Σ, ind_universes mdecl)
+          mdecl (inductive_ind ind) idecl (ind_indices oib) cdecl cshape),
+  wf_global_ext Σ (ind_universes mdecl) *
+  wf_local (Σ, ind_universes mdecl)
+   (arities_context (ind_bodies mdecl) ,,, ind_params mdecl ,,, cshape_args cshape) *
+  ctx_inst (Σ, ind_universes mdecl)
+             (arities_context (ind_bodies mdecl) ,,, ind_params mdecl ,,,
+              cshape_args cshape)
+             (cshape_indices cshape) 
+            (List.rev (lift_context #|cshape_args cshape| 0 (ind_indices oib))). 
+Proof.
+  move=> wfΣ declm oi oib onc.
+  pose proof (on_cargs onc). simpl in X.
+  split.
+  - split. split.
+    2:{ eapply (weaken_lookup_on_global_env'' _ _ (InductiveDecl mdecl)); pcuic. destruct declm; pcuic. }
+    red. split; eauto. simpl. eapply (weaken_lookup_on_global_env' _ _ (InductiveDecl mdecl)); eauto.
+    destruct declm; pcuic.
+    eapply type_local_ctx_wf_local in X => //. clear X.
+    eapply weaken_wf_local => //.
+    eapply wf_arities_context; eauto. destruct declm; eauto.
+    now eapply onParams.
+  - apply (on_cindices onc).
+Qed.
+
+Lemma on_constructor_subst {cf:checker_flags} Σ ind mdecl idecl cshape cdecl : 
+  wf Σ -> 
+  declared_inductive Σ mdecl ind idecl ->
+  on_inductive (lift_typing typing) (Σ, ind_universes mdecl) (inductive_mind ind) mdecl ->
+  forall (oib : on_ind_body (lift_typing typing) (Σ, ind_universes mdecl) (inductive_mind ind) mdecl 
+           (inductive_ind ind) idecl)
+        (onc : on_constructor (lift_typing typing) (Σ, ind_universes mdecl)
+          mdecl (inductive_ind ind) idecl (ind_indices oib) cdecl cshape),
+  wf_global_ext Σ (ind_universes mdecl) *
+  wf_local (Σ, ind_universes mdecl)
+   (arities_context (ind_bodies mdecl) ,,, ind_params mdecl ,,, cshape_args cshape) *
+  ∑ inst,
+  spine_subst (Σ, ind_universes mdecl)
+             (arities_context (ind_bodies mdecl) ,,, ind_params mdecl ,,,
+              cshape_args cshape)
+             ((to_extended_list_k (ind_params mdecl) #|cshape_args cshape|) ++
+              (cshape_indices cshape)) inst
+          (ind_params mdecl ,,, ind_indices oib). 
+Proof.
+  move=> wfΣ declm oi oib onc.
+  pose proof (onc.(on_cargs)). simpl in X.
+  split. split. split.
+  2:{ eapply (weaken_lookup_on_global_env'' _ _ (InductiveDecl mdecl)); pcuic. destruct declm; pcuic. }
+  red. split; eauto. simpl. eapply (weaken_lookup_on_global_env' _ _ (InductiveDecl mdecl)); eauto.
+  destruct declm; pcuic. 
+  eapply type_local_ctx_wf_local in X => //. clear X.
+  eapply weaken_wf_local => //.
+  eapply wf_arities_context; eauto. destruct declm; eauto.
+  now eapply onParams.
+  destruct (on_ctype onc).
+  rewrite onc.(cstr_eq) in t.
+  rewrite -it_mkProd_or_LetIn_app in t.
+  eapply inversion_it_mkProd_or_LetIn in t => //.
+  unfold cstr_concl_head in t. simpl in t.
+  eapply inversion_mkApps in t as [A [ta sp]].
+  eapply inversion_Rel in ta as [decl [wfΓ [nth cum']]].
+  rewrite nth_error_app_ge in nth. autorewrite with len. lia.
+  autorewrite with len in nth.
+  all:auto.
+  assert ( (#|ind_bodies mdecl| - S (inductive_ind ind) + #|ind_params mdecl| +
+  #|cshape_args cshape| -
+  (#|cshape_args cshape| + #|ind_params mdecl|)) = #|ind_bodies mdecl| - S (inductive_ind ind)) by lia.
+  move: nth; rewrite H; clear H. destruct nth_error eqn:Heq => //.
+  simpl.
+  move=> [=] Hdecl. eapply (nth_errror_arities_context (Σ, ind_universes mdecl)) in Heq; eauto.
+  subst decl.
+  rewrite Heq in cum'; clear Heq c.
+  assert(closed (ind_type idecl)).
+  { pose proof (oib.(onArity)). rewrite (oib.(ind_arity_eq)) in X0 |- *.
+    destruct X0 as [s Hs]. now apply subject_closed in Hs. } 
+  rewrite lift_closed in cum' => //.
+  eapply typing_spine_strengthen in sp; pcuic.
+  move: sp. 
+  rewrite (oib.(ind_arity_eq)).
+  rewrite -it_mkProd_or_LetIn_app.
+  move=> sp. simpl in sp.
+  apply (arity_typing_spine (Σ, ind_universes mdecl)) in sp as [[Hlen Hleq] [inst Hinst]] => //.
+  clear Hlen.
+  rewrite [_ ,,, _]app_context_assoc in Hinst.
+  now exists inst.
+  apply weaken_wf_local => //.
+
+  rewrite [_ ,,, _]app_context_assoc in wfΓ.
+  eapply All_local_env_app in wfΓ as [? ?].
+  apply on_minductive_wf_params_indices => //. pcuic.
+Qed.
+
+Lemma on_constructor_inst {cf:checker_flags} Σ ind u mdecl idecl cshape cdecl : 
+  wf Σ.1 -> 
+  declared_inductive Σ.1 mdecl ind idecl ->
+  on_inductive (lift_typing typing) (Σ.1, ind_universes mdecl) (inductive_mind ind) mdecl ->
+  forall (oib : on_ind_body (lift_typing typing) (Σ.1, ind_universes mdecl) (inductive_mind ind) mdecl 
+           (inductive_ind ind) idecl)
+        (onc : on_constructor (lift_typing typing) (Σ.1, PCUICAst.ind_universes mdecl)
+          mdecl (inductive_ind ind) idecl (ind_indices oib) cdecl cshape), 
+  consistent_instance_ext Σ (ind_universes mdecl) u ->
+  wf_local Σ (subst_instance_context u
+    (arities_context (ind_bodies mdecl) ,,, ind_params mdecl ,,, cshape_args cshape)) *
+  ∑ inst,
+  spine_subst Σ
+          (subst_instance_context u
+             (arities_context (ind_bodies mdecl) ,,, ind_params mdecl ,,,
+              cshape_args cshape))
+          (map (subst_instance_constr u)
+             (to_extended_list_k (ind_params mdecl) #|cshape_args cshape|) ++
+           map (subst_instance_constr u) (cshape_indices cshape)) inst
+          (subst_instance_context u (ind_params mdecl) ,,,
+           subst_instance_context u (ind_indices oib)). 
+Proof.
+  move=> wfΣ declm oi oib onc cext.
+  destruct (on_constructor_subst Σ.1 ind mdecl idecl _ cdecl wfΣ declm oi oib onc) as [[wfext wfl] [inst sp]].
+  eapply wf_local_subst_instance in wfl; eauto. split=> //.
+  eapply spine_subst_inst in sp; eauto.
+  rewrite map_app in sp. rewrite -subst_instance_context_app.
+  eexists ; eauto.
+Qed.
+
+Lemma mkApps_ind_typing_spine {cf:checker_flags} Σ Γ Γ' ind i
+  inst ind' i' args args' : 
+  wf Σ.1 ->
+  wf_local Σ Γ ->
+  isWfArity_or_Type Σ Γ (it_mkProd_or_LetIn Γ' (mkApps (tInd ind i) args)) ->
+  typing_spine Σ Γ (it_mkProd_or_LetIn Γ' (mkApps (tInd ind i) args)) inst 
+    (mkApps (tInd ind' i') args') ->
+  ∑ instsubst, (make_context_subst (List.rev Γ') inst [] = Some instsubst) *
+  (#|inst| = context_assumptions Γ' /\ ind = ind' /\ 
+  R_universe_instance (eq_universe (global_ext_constraints Σ)) i i') *
+  All2 (fun par par' => Σ ;;; Γ |- par = par') (map (subst0 instsubst) args) args' *
+  (subslet Σ Γ instsubst Γ').
+Proof.
+  intros wfΣ wfΓ; revert args args' ind i ind' i' inst.
+  revert Γ'. refine (ctx_length_rev_ind _ _ _); simpl.
+  - intros args args' ind i ind' i' inst wat Hsp.
+    depelim Hsp.
+    eapply invert_cumul_ind_l in c as [i'' [args'' [? ?]]]; auto.
+    eapply red_mkApps_tInd in r as [? [eq ?]]; auto. solve_discr.
+    exists nil.
+    intuition auto. clear i0.
+    revert args' a. clear -b wfΣ wfΓ. induction b; intros args' H; depelim H; constructor.
+    rewrite subst_empty.
+    transitivity y; auto. symmetry.
+    now eapply red_conv. now eauto.
+    eapply invert_cumul_prod_r in c as [? [? [? [[? ?] ?]]]]; auto.
+    eapply red_mkApps_tInd in r as [? [eq ?]]; auto. now solve_discr.
+  - intros d Γ' IH args args' ind i ind' i' inst wat Hsp.
+    rewrite it_mkProd_or_LetIn_app in Hsp.
+    destruct d as [na [b|] ty]; simpl in *; rewrite /mkProd_or_LetIn /= in Hsp.
+    + rewrite context_assumptions_app /= Nat.add_0_r.
+      eapply typing_spine_letin_inv in Hsp; auto.
+      rewrite /subst1 subst_it_mkProd_or_LetIn /= in Hsp.
+      specialize (IH (subst_context [b] 0 Γ')).
+      forward IH by rewrite subst_context_length; lia.
+      rewrite subst_mkApps Nat.add_0_r in Hsp.
+      specialize (IH (map (subst [b] #|Γ'|) args) args' ind i ind' i' inst).
+      forward IH. {
+        move: wat; rewrite it_mkProd_or_LetIn_app /= /mkProd_or_LetIn /= => wat.
+        eapply isWAT_tLetIn_red in wat; auto.
+        now rewrite /subst1 subst_it_mkProd_or_LetIn subst_mkApps Nat.add_0_r
+        in wat. }
+      rewrite context_assumptions_subst in IH.
+      intuition auto.
+      destruct X as [isub [[[Hisub Hinst] Hargs] Hs]].
+      eexists. intuition auto.
+      eapply make_context_subst_spec in Hisub.
+      eapply make_context_subst_spec_inv.
+      rewrite List.rev_app_distr. simpl.
+      rewrite List.rev_involutive.
+      eapply (context_subst_subst [{| decl_name := na; decl_body := Some b;  decl_type := ty |}] [] [b] Γ').
+      rewrite -{2}  (subst_empty 0 b). eapply context_subst_def. constructor.
+      now rewrite List.rev_involutive in Hisub.
+      rewrite map_map_compose in Hargs.
+      assert (map (subst0 isub ∘ subst [b] #|Γ'|) args = map (subst0 (isub ++ [b])) args) as <-.
+      { eapply map_ext => x. simpl.
+        assert(#|Γ'| = #|isub|).
+        { apply make_context_subst_spec in Hisub.
+          apply context_subst_length in Hisub.
+          now rewrite List.rev_involutive subst_context_length in Hisub. }
+        rewrite H0.
+        now rewrite -(subst_app_simpl isub [b] 0). }
+      exact Hargs. 
+      eapply subslet_app; eauto. rewrite -{1}(subst_empty 0 b). repeat constructor.
+      rewrite !subst_empty.
+      rewrite it_mkProd_or_LetIn_app /= /mkProd_or_LetIn /= in wat.
+      now eapply isWAT_tLetIn_dom in wat.
+    + rewrite context_assumptions_app /=.
+      pose proof (typing_spine_WAT_concl Hsp).
+      depelim Hsp.
+      eapply invert_cumul_prod_l in c as [? [? [? [[? ?] ?]]]]; auto.
+      eapply red_mkApps_tInd in r as [? [eq ?]]; auto. now solve_discr.
+      eapply cumul_Prod_inv in c as [conva cumulB].
+      eapply (substitution_cumul0 _ _ _ _ _ _ hd) in cumulB; auto.
+      rewrite /subst1 subst_it_mkProd_or_LetIn /= in cumulB.
+      specialize (IH (subst_context [hd] 0 Γ')).
+      forward IH by rewrite subst_context_length; lia.
+      specialize (IH (map (subst [hd] #|Γ'|) args) args' ind i ind' i' tl). all:auto.
+      have isWATs: isWfArity_or_Type Σ Γ
+      (it_mkProd_or_LetIn (subst_context [hd] 0 Γ')
+          (mkApps (tInd ind i) (map (subst [hd] #|Γ'|) args))). {
+        move: wat; rewrite it_mkProd_or_LetIn_app /= /mkProd_or_LetIn /= => wat.
+        eapply isWAT_tProd in wat; auto. destruct wat as [isty wat].
+        epose proof (isWAT_subst wfΣ (Γ:=Γ) (Δ:=[vass na ty])).
+        forward X0. constructor; auto.
+        specialize (X0 (it_mkProd_or_LetIn Γ' (mkApps (tInd ind i) args)) [hd]).
+        forward X0. constructor. constructor. rewrite subst_empty; auto.
+        eapply isWAT_tProd in i0; auto. destruct i0. 
+        eapply type_Cumul with A; auto. now eapply conv_cumul.
+        now rewrite /subst1 subst_it_mkProd_or_LetIn subst_mkApps Nat.add_0_r
+        in X0. }
+      rewrite subst_mkApps Nat.add_0_r in cumulB. simpl in *. 
+      rewrite context_assumptions_subst in IH.
+      eapply typing_spine_strengthen in Hsp.
+      3:eapply cumulB. all:eauto.
+      intuition auto.
+      destruct X1 as [isub [[[Hisub [Htl [Hind Hu]]] Hargs] Hs]].
+      exists (isub ++ [hd])%list. rewrite List.rev_app_distr.
+      intuition auto. 2:lia.
+      * apply make_context_subst_spec_inv.
+        apply make_context_subst_spec in Hisub.
+        rewrite List.rev_app_distr !List.rev_involutive in Hisub |- *.
+        eapply (context_subst_subst [{| decl_name := na; decl_body := None; decl_type := ty |}] [hd] [hd] Γ'); auto.
+        eapply (context_subst_ass _ [] []). constructor.
+      * assert (map (subst0 isub ∘ subst [hd] #|Γ'|) args = map (subst0 (isub ++ [hd])) args) as <-.
+      { eapply map_ext => x. simpl.
+        assert(#|Γ'| = #|isub|).
+        { apply make_context_subst_spec in Hisub.
+          apply context_subst_length in Hisub.
+          now rewrite List.rev_involutive subst_context_length in Hisub. }
+        rewrite H.
+        now rewrite -(subst_app_simpl isub [hd] 0). }
+        now rewrite map_map_compose in Hargs.
+      * eapply subslet_app; auto.
+        constructor. constructor. rewrite subst_empty.
+        rewrite it_mkProd_or_LetIn_app /= /mkProd_or_LetIn /= in wat.
+        eapply isWAT_tProd in wat as [Hty _]; auto.
+        eapply type_Cumul; eauto. now eapply conv_cumul.
+Qed.
+
+Lemma Construct_Ind_ind_eq {cf:checker_flags} {Σ} (wfΣ : wf Σ.1):
+  forall {Γ n i args u i' args' u' mdecl idecl cdecl},
+  Σ ;;; Γ |- mkApps (tConstruct i n u) args : mkApps (tInd i' u') args' ->
+  forall (Hdecl : declared_constructor Σ.1 mdecl idecl (i, n) cdecl),
+  let '(onind, oib, existT cshape (hnth, onc)) := on_declared_constructor wfΣ Hdecl in
+  (i = i') * 
+  (* Universe instances match *)
+  R_universe_instance (eq_universe (global_ext_constraints Σ)) u u' *
+  consistent_instance_ext Σ (ind_universes mdecl) u' *    
+  (#|args| = (ind_npars mdecl + context_assumptions cshape.(cshape_args))%nat) *
+  ∑ parsubst argsubst parsubst' argsubst',
+    let parctx := (subst_instance_context u (ind_params mdecl)) in
+    let parctx' := (subst_instance_context u' (ind_params mdecl)) in
+    let argctx := (subst_context parsubst 0
+    ((subst_context (inds (inductive_mind i) u mdecl.(ind_bodies)) #|ind_params mdecl|
+    (subst_instance_context u cshape.(cshape_args))))) in
+    let argctx' := (subst_context parsubst' 0 (subst_instance_context u' oib.(ind_indices))) in
+    
+    spine_subst Σ Γ (firstn (ind_npars mdecl) args) parsubst parctx *
+    spine_subst Σ Γ (firstn (ind_npars mdecl) args') parsubst' parctx' *
+    spine_subst Σ Γ (skipn (ind_npars mdecl) args) argsubst argctx *
+    spine_subst Σ Γ (skipn (ind_npars mdecl) args')  argsubst' argctx' *
+
+    ∑ s, type_local_ctx (lift_typing typing) Σ Γ argctx s *
+    (** Parameters match *)
+    (All2 (fun par par' => Σ ;;; Γ |- par = par') 
+      (firstn mdecl.(ind_npars) args) 
+      (firstn mdecl.(ind_npars) args') * 
+
+    (** Indices match *)
+    All2 (fun par par' => Σ ;;; Γ |- par = par') 
+      (map (subst0 (argsubst ++ parsubst) ∘ 
+      subst (inds (inductive_mind i) u mdecl.(ind_bodies)) (#|cshape.(cshape_args)| + #|ind_params mdecl|)
+      ∘ (subst_instance_constr u)) 
+        cshape.(cshape_indices))
+      (skipn mdecl.(ind_npars) args')).
+
+Proof.
+  intros Γ n i args u i' args' u' mdecl idecl cdecl h declc.
+  unfold on_declared_constructor.
+  destruct (on_declared_constructor _ declc). destruct s as [? [_ onc]].
+  unshelve epose proof (env_prop_typing _ _ validity _ _ _ _ _ h) as vi'; eauto using typing_wf_local.
+  eapply inversion_mkApps in h; auto.
+  destruct h as [T [hC hs]].
+  apply inversion_Construct in hC
+    as [mdecl' [idecl' [cdecl' [hΓ [isdecl [const htc]]]]]]; auto.
+  assert (vty:=declared_constructor_valid_ty _ _ _ _ _ _ _ _ wfΣ hΓ isdecl const). 
+  eapply typing_spine_strengthen in hs. 3:eapply htc. all:eauto.
+  destruct (declared_constructor_inj isdecl declc) as [? [? ?]].
+  subst mdecl' idecl' cdecl'. clear isdecl.
+  destruct p as [onmind onind]. clear onc.
+  destruct declc as [decli declc].
+  remember (on_declared_inductive wfΣ decli). clear onmind onind.
+  destruct p.
+  rename o into onmind. rename o0 into onind.
+  destruct declared_constructor_inv as [cshape [_ onc]].
+  simpl in onc. unfold on_declared_inductive in Heqp.
+  injection Heqp. intros indeq _. 
+  move: onc Heqp. rewrite -indeq.
+  intros onc Heqp. clear Heqp. simpl in onc.
+  pose proof (on_constructor_inst _ _ _ _ _ _ _ wfΣ decli onmind onind onc const).
+  destruct onc as [argslength conclhead cshape_eq [cs' t] cargs cinds]; simpl.
+  simpl in *. 
+  unfold type_of_constructor in hs. simpl in hs.
+  unfold cdecl_type in cshape_eq.
+  rewrite cshape_eq in hs.  
+  rewrite !subst_instance_constr_it_mkProd_or_LetIn in hs.
+  rewrite !subst_it_mkProd_or_LetIn subst_instance_context_length Nat.add_0_r in hs.
+  rewrite subst_instance_constr_mkApps subst_mkApps subst_instance_context_length in hs.
+  assert (Hind : inductive_ind i < #|ind_bodies mdecl|).
+  { red in decli. destruct decli. clear -e.
+    now eapply nth_error_Some_length in e. }
+  rewrite (subst_inds_concl_head i) in hs => //.
+  rewrite -it_mkProd_or_LetIn_app in hs.
+  assert(ind_npars mdecl = PCUICAst.context_assumptions (ind_params mdecl)).
+  { now pose (onNpars _ _ _ _ onmind). }
+  assert (closed_ctx (ind_params mdecl)).
+  { destruct onmind.
+    red in onParams. now apply closed_wf_local in onParams. }
+  eapply mkApps_ind_typing_spine in hs as [isubst [[[Hisubst [Hargslen [Hi Hu]]] Hargs] Hs]]; auto.
+  subst i'.
+  eapply (isWAT_mkApps_Ind wfΣ decli) in vi' as (parsubst & argsubst & (spars & sargs) & cons) => //.
+  unfold on_declared_inductive in sargs. simpl in sargs. rewrite -indeq in sargs. clear indeq.
+  split=> //. split=> //.
+  now rewrite Hargslen context_assumptions_app !context_assumptions_subst !subst_instance_context_assumptions; lia.
+
+  exists (skipn #|cshape.(cshape_args)| isubst), (firstn #|cshape.(cshape_args)| isubst).
+  apply make_context_subst_spec in Hisubst.
+  move: Hisubst.
+  rewrite List.rev_involutive.
+  move/context_subst_app.
+  rewrite !subst_context_length !subst_instance_context_length.
+  rewrite context_assumptions_subst subst_instance_context_assumptions -H.
+  move=>  [argsub parsub].
+  rewrite closed_ctx_subst in parsub.
+  now rewrite closedn_subst_instance_context.
+  eapply subslet_app_inv in Hs.
+  move: Hs. autorewrite with len. intuition auto.
+  rewrite closed_ctx_subst in a0 => //.
+  now rewrite closedn_subst_instance_context.
+
+  (*rewrite -Heqp in spars sargs. simpl in *. clear Heqp. *)
+  exists parsubst, argsubst.
+  assert(wfar : wf_local Σ
+  (Γ ,,, subst_instance_context u (arities_context (ind_bodies mdecl)))).
+  { eapply weaken_wf_local => //.
+    eapply wf_local_instantiate => //; destruct decli; eauto.
+    eapply wf_arities_context => //; eauto. }
+  assert(wfpars : wf_local Σ (subst_instance_context u (ind_params mdecl))).
+    { eapply on_minductive_wf_params => //; eauto.
+      destruct decli; eauto. }
+      
+  intuition auto; try split; auto.
+  - apply weaken_wf_local => //.
+  - pose proof (subslet_length a0). rewrite subst_instance_context_length in H1.
+    rewrite -H1 -subst_app_context.
+    eapply (substitution_wf_local _ _ (subst_instance_context u (arities_context (ind_bodies mdecl) ,,, ind_params mdecl))); eauto.
+    rewrite subst_instance_context_app; eapply subslet_app; eauto.
+    now rewrite closed_ctx_subst ?closedn_subst_instance_context.
+    eapply (weaken_subslet _ _ _ _ []) => //.
+    now eapply subslet_inds; eauto.
+    rewrite -app_context_assoc.
+    eapply weaken_wf_local => //.
+    rewrite -subst_instance_context_app. 
+    apply a.
+  - exists (subst_instance_univ u (cshape_sort cshape)). split.
+    move/onParams: onmind. rewrite /on_context.
+    pose proof (wf_local_instantiate Σ (InductiveDecl mdecl) (ind_params mdecl) u).
+    move=> H'. eapply X in H'; eauto.
+    2:destruct decli; eauto.
+    clear -wfar wfpars wfΣ hΓ const decli t cargs H0 H' a a0.
+    eapply (subst_type_local_ctx _ _ [] 
+      (subst_context (inds (inductive_mind i) u (ind_bodies mdecl)) 0 (subst_instance_context u (ind_params mdecl)))) => //.
+    simpl. eapply weaken_wf_local => //.
+    rewrite closed_ctx_subst => //.
+    now rewrite closedn_subst_instance_context.
+    simpl. rewrite -(subst_instance_context_length u (ind_params mdecl)).
+    eapply (subst_type_local_ctx _ _ _ (subst_instance_context u (arities_context (ind_bodies mdecl)))) => //.
+    eapply weaken_wf_local => //.
+    rewrite -app_context_assoc.
+    eapply weaken_type_local_ctx => //.
+    rewrite -subst_instance_context_app.
+    eapply type_local_ctx_instantiate => //; destruct decli; eauto.
+    eapply (weaken_subslet _ _ _ _ []) => //.
+    now eapply subslet_inds; eauto.
+    now rewrite closed_ctx_subst ?closedn_subst_instance_context.
+
+    move: (All2_firstn  _ _ _ _ _ mdecl.(ind_npars) Hargs).
+    move: (All2_skipn  _ _ _ _ _ mdecl.(ind_npars) Hargs).
+    clear Hargs.
+    rewrite !map_map_compose !map_app.
+    rewrite -map_map_compose.
+    rewrite (firstn_app_left _ 0).
+    { rewrite !map_length to_extended_list_k_length. lia. }
+    rewrite /= app_nil_r.
+    rewrite skipn_all_app_eq.
+    autorewrite with len. 
+    rewrite to_extended_list_k_length. lia.
+    rewrite !map_map_compose.
+    assert (#|cshape.(cshape_args)| <= #|isubst|).
+    apply context_subst_length in argsub.
+    autorewrite with len in argsub.
+    now apply firstn_length_le_inv.
+
+    rewrite -(firstn_skipn #|cshape.(cshape_args)| isubst).
+    rewrite -[map _ (to_extended_list_k _ _)]
+               (map_map_compose _ _ _ (subst_instance_constr u)
+                              (fun x => subst _ _ (subst _ _ x))).
+    rewrite subst_instance_to_extended_list_k.
+    rewrite -[map _ (to_extended_list_k _ _)]map_map_compose. 
+    rewrite -to_extended_list_k_map_subst.
+    rewrite subst_instance_context_length. lia.
+    rewrite map_subst_app_to_extended_list_k.
+    rewrite firstn_length_le => //.
+    
+    erewrite subst_to_extended_list_k.
+    rewrite map_lift0. split. eauto.
+    rewrite firstn_skipn. rewrite firstn_skipn in All2_skipn.
+    now rewrite firstn_skipn.
+
+    apply make_context_subst_spec_inv. now rewrite List.rev_involutive.
+
+  - rewrite it_mkProd_or_LetIn_app.
+    right. unfold type_of_constructor in vty.
+    rewrite cshape_eq in vty. move: vty.
+    rewrite !subst_instance_constr_it_mkProd_or_LetIn.
+    rewrite !subst_it_mkProd_or_LetIn subst_instance_context_length Nat.add_0_r.
+    rewrite subst_instance_constr_mkApps subst_mkApps subst_instance_context_length.
+    rewrite subst_inds_concl_head. all:simpl; auto.
+Qed.
+
+Notation "⋆" := ltac:(solve [pcuic]) (only parsing).
+
+Lemma build_branches_type_red {cf:checker_flags} (p p' : term) (ind : inductive)
+	(mdecl : PCUICAst.mutual_inductive_body)
+    (idecl : PCUICAst.one_inductive_body) (pars : list term) 
+    (u : Instance.t) (brtys : list (nat × term)) Σ Γ :
+  wf Σ ->
+  red1 Σ Γ p p' ->
+  map_option_out (build_branches_type ind mdecl idecl pars u p) = Some brtys ->
+  ∑ brtys' : list (nat × term),
+    map_option_out (build_branches_type ind mdecl idecl pars u p') =
+    Some brtys' × All2 (on_Trel_eq (red1 Σ Γ) snd fst) brtys brtys'.
+Proof.
+  intros wfΣ redp.
+  unfold build_branches_type.
+  unfold mapi.
+  generalize 0 at 3 6.
+  induction (ind_ctors idecl) in brtys |- *. simpl.
+  intros _ [= <-]. exists []; split; auto.
+  simpl. intros n.
+  destruct a. destruct p0.
+  destruct (instantiate_params (subst_instance_context u (PCUICAst.ind_params mdecl))
+  pars
+  (subst0 (inds (inductive_mind ind) u (PCUICAst.ind_bodies mdecl))
+     (subst_instance_constr u t))).
+  destruct decompose_prod_assum.
+  destruct chop.
+  destruct map_option_out eqn:Heq.
+  specialize (IHl _ _ Heq).
+  destruct IHl. intros [= <-].
+  exists ((n0,
+  PCUICAst.it_mkProd_or_LetIn c
+    (mkApps (lift0 #|c| p')
+       (l1 ++
+        [mkApps (tConstruct ind n u) (l0 ++ PCUICAst.to_extended_list c)]))) :: x).
+  destruct p0 as [l' r'].
+  rewrite {}l'.
+  split; auto.
+  constructor; auto. simpl. split; auto.
+  2:discriminate. clear Heq.
+  2:discriminate.
+  eapply red1_it_mkProd_or_LetIn.
+  eapply red1_mkApps_f.
+  eapply (weakening_red1 Σ Γ [] c) => //.
+Qed.
+
+Lemma conv_decls_fix_context_gen {cf:checker_flags} Σ Γ mfix mfix1 :
+  wf Σ.1 ->
+  All2 (fun d d' => conv Σ Γ d.(dtype) d'.(dtype)) mfix mfix1 ->
+  forall Γ' Γ'',
+  conv_context Σ (Γ ,,, Γ') (Γ ,,, Γ'') ->
+  context_relation (fun Δ Δ' : PCUICAst.context => conv_decls Σ (Γ ,,, Γ' ,,, Δ) (Γ ,,, Γ'' ,,, Δ'))
+    (fix_context_gen #|Γ'| mfix) (fix_context_gen #|Γ''| mfix1).
+Proof.    
+  intros wfΣ.
+  induction 1. constructor. simpl.
+  intros Γ' Γ'' convctx.
+
+  assert(conv_decls Σ (Γ ,,, Γ' ,,, []) (Γ ,,, Γ'' ,,, [])
+  (PCUICAst.vass (dname x) (lift0 #|Γ'| (dtype x)))
+  (PCUICAst.vass (dname y) (lift0 #|Γ''| (dtype y)))).
+  { constructor.
+  pose proof (context_relation_length _ _ _  convctx).
+  rewrite !app_length in H. assert(#|Γ'|  = #|Γ''|) by lia.
+  rewrite -H0.
+  apply (weakening_conv _ _ []); auto. }
+
+  apply context_relation_app_inv. rewrite !List.rev_length; autorewrite with len.
+  now apply All2_length in X.
+  constructor => //.
+  eapply (context_relation_impl (P:= (fun Δ Δ' : PCUICAst.context =>
+  conv_decls Σ
+  (Γ ,,, (vass (dname x) (lift0 #|Γ'| (dtype x)) :: Γ') ,,, Δ)
+  (Γ ,,, (vass (dname y) (lift0 #|Γ''| (dtype y)) :: Γ'') ,,, Δ')))).
+  intros. now rewrite !app_context_assoc.
+  eapply IHX. simpl.
+  constructor => //.
+Qed.
+
+Lemma conv_decls_fix_context {cf:checker_flags} Σ Γ mfix mfix1 :
+  wf Σ.1 ->
+  All2 (fun d d' => conv Σ Γ d.(dtype) d'.(dtype)) mfix mfix1 ->
+  context_relation (fun Δ Δ' : PCUICAst.context => conv_decls Σ (Γ ,,, Δ) (Γ ,,, Δ'))
+    (fix_context mfix) (fix_context mfix1).
+Proof.    
+  intros wfΣ a.
+  apply (conv_decls_fix_context_gen _ _  _ _ wfΣ a [] []).
+  apply conv_ctx_refl. 
+Qed.
+
+Lemma isLambda_red1 Σ Γ b b' : isLambda b -> red1 Σ Γ b b' -> isLambda b'.
+Proof.
+  destruct b; simpl; try discriminate.
+  intros _ red.
+  depelim red.
+  symmetry in H; apply mkApps_Fix_spec in H. simpl in H. intuition.
+  constructor. constructor.
+Qed.
